Fixing prf-prp example

theories/ub_logic/ub_examples.v
@@ -2,7 +2,7 @@ From clutch.ub_logic Require Export ub_clutch.
 
 
 Local Open Scope R.
-Context `{!clutchGS Σ}.
+Context `{!ub_clutchGS Σ}.
 
 Definition foo N (m : nat) : expr :=
   let: "n" := rand #N from #() in
@@ -52,3 +52,57 @@ Proof.
   wp_if_false.
   by iApply "HΦ".
 Qed.
+
+
+Definition baz : expr :=
+  rec: "baz" "x" :=
+    let: "n" := rand #2 from #() in
+    (if: "n" < #2
+      then "n"
+      else "baz" #() ).
+
+
+Lemma wp_baz E :
+  € (nnreal_inv (nnreal_nat 2)) -∗ WP baz #() @ E {{ v, ⌜v = #0⌝ }}.
+Proof.
+  iIntros "Herr".
+  wp_pure.
+  iLöb as "IH".
+  wp_pures.
+  set f:= (λ n : fin 3,
+              if bool_decide (n = 0%fin)
+                then nnreal_zero
+                else if bool_decide (n = 1%fin) then nnreal_one
+                                            else nnreal_inv((nnreal_nat 2))).
+  unshelve wp_apply (wp_couple_rand_adv_comp _ _ _ _ _ f with "Herr").
+  { intro. exact ⌜ true ⌝%I. }.
+  {
+    exists 1; intro n.
+    rewrite /f.
+    case_bool_decide.
+    - simpl; lra.
+    - case_bool_decide; simpl; lra.
+  }
+  {
+    admit.
+  }
+  iIntros (n) "Hεcont".
+  wp_pures.
+  case_bool_decide.
+  - destruct (decide (n = 0%fin)) as [->|].
+    + wp_pures. done.
+    + assert (n = 1%fin) as ->.
+      {
+        admit.
+      }
+      rewrite /f/=.
+      (* Should be allowed to prove this for free with €1 *)
+      admit.
+  - assert (n = 2%fin) as ->; [admit|].
+    wp_pure.
+    iApply "IH".
+    rewrite /f/=.
+    done.
+Admitted.
+
+
